\documentclass[a4paper]{article}

\title{Solutions to Recitation 2}
\author{L. F. \textsc{Jaw}}

\input{preamble-all}
\input{preamble-en}
\input{preamble-begin}

\begin{document}
\maketitle

This is my own solution to the recitation 2 of
\href{https://ocw.mit.edu/courses/mathematics/18-014-calculus-with-theory-fall-2010/recitations/}{18.014},
which includes Theorem I.9-10 and Exercise 4 from Apostol's
\emph{Calculus} (1: 18-19).

\pskip

The cancellation law (Theorem I.7) implies the uniqueness of the
inverse if it exists and thus we use the notation \(a^{-1}\)
introduced in the Theorem I.8 freely without any ambiguity.
Furthermore, if \(a \ne 0\), then \(a^{-1} \ne 0\).  If otherwise,
\(a \cdot a^{-1} = a \cdot 0 = 0 \ne 1\).

\begin{enumerate}
\item If \(a \ne 0\), then \(b/a = b \cdot a^{-1}\).

  We have
  \begin{align*}
    a \cdot \paren{b/a}
    &= b                        && \reason{by definition of division,} \\
    &= 1 \cdot b                && \reason{by the identity axiom,}\\
    &= \paren{aa^{-1}} \cdot b  && \reason{by the inverse axiom,} \\
    &= a \cdot \paren{a^{-1} b} && \reason{by associativity,} \\
    &= a \cdot \paren{ba^{-1}}  && \reason{by commutativity.}
  \end{align*}
  We apply the cancellation law (Theorem I.7) to the above and obtain
  \(b/a = b \cdot a^{-1}\).  \qed

\item If \(a \ne 0\), then \(\paren{a^{-1}}^{-1} = a\).

  Since \(a \ne 0\), \(a^{-1} \ne 0\).  And we have
  \begin{align*}
    a^{-1} \cdot \paren{a^{-1}}^{-1}
    &= 1              && \reason{by definition of reciprocal,} \\
    &= a \cdot a^{-1} && \reason{by the inverse axiom,} \\
    &= a^{-1} \cdot a && \reason{by commutativity.}
  \end{align*}
  By the cancellation law, we obtain \(\paren{a^{-1}}^{-1} = a\).  \qed

\item Zero has no reciprocal.

  Suppose zero has a reciprocal and let us denote it as \(0^{-1}\).  Then
  \begin{align*}
    0 &= 0 \cdot 0^{-1} && \reason{by Theorem I.6,} \\
      &= 1              && \reason{by definition of reciprocal.}
  \end{align*}
  But by the identity axoim, \(0 \ne 1\).  This is contradictory.  \qed
\end{enumerate}

\end{document}
