\documentclass[a4paper]{article}

\title{Solutions to Recitation~4}
\author{L. F. \textsc{Jaw}}

\input{preamble-all}
\input{preamble-en}
\input{preamble-begin}

\begin{document}
\maketitle

This is my own solution to the Recitation~4 of
\href{https://ocw.mit.edu/courses/mathematics/18-014-calculus-with-theory-fall-2010/recitations/}{18.014},
which includes Exercise~3 from Munkres's Course Note~A and Exercise~3 and
1achi from Apostol's \textit{Calculus} (9; 1: 28, 43).

\begin{enumerate}
\item Show that if a set \(A\) of integers is bounded above, then
  \(A\) has a largest element.

  \begin{proof}
    By the least-upper-bound axiom, there exists a real number \(u\) such
    that \(u = \sup A\).  If \(u \in A\), we are done since \(u\) is the
    largest element.  If \(u \notin A\), then by definition there must
    exist an integer \(n \in A\) such that \(u-1 < n < u\).  The last
    inequality is the same as \(u < n+1 < u+1\).  If \(n+1 \in A\), then
    \(u\) is not a upper bound for \(A\).  It follows that \(k \notin A\)
    for all integers \(k \ge n+1\).  Then we find the largest element in
    \(A\), which is simply \(n\).  (Furthermore, \(u = n\).)
  \end{proof}

\item If \(x > 0\), prove that there is a positive integer \(n\) such that
  \(1/n < x\).

  \begin{proof}
    Simply apply Theorem~I.30 with \(y = 1\) and we have \(nx > 1\).
    Divide both side of the inequality with \(n\) and we obtain
    \(1/n < x\).
  \end{proof}

\item Prove each of the following properties of absolute values.
  \begin{enumerate}
  \item \(\abs{x} = 0\) if and only if \(x = 0\).

    \begin{proof}
      If \(\abs{x} = 0\), then either \(x = -\abs{x} = -0\) or
      \(x = \abs{x} = 0\).  In both cases, we have \(x = 0\).  If
      \(x = 0\), then clearly we have \(\abs{x} = x = -x = 0\).
    \end{proof}

  \item \(\abs{x-y} = \abs{y-x}\).

    \begin{proof}
      We have \(\abs{x-y} = \abs{-(y-x)} = \abs{y-x}\).
    \end{proof}

  \item \(\abs{x-y} \le \abs{x} + \abs{y}\).

    \begin{proof}
      We have
      \begin{align*}
        \abs{x-y} &= \abs{x+(-y)} \\
                  &\le \abs{x} + \abs{-y} \\
                  &=\abs{x} + \abs{y}. \qedhere
      \end{align*}
    \end{proof}

  \item \(\abs{x} - \abs{y} \le \abs{x-y}\).

    \begin{proof}
      We have
      \begin{align*}
        \abs{x} &= \abs{x - y + y} \\
                &\le \abs{x-y} + \abs{y}.
      \end{align*}
      Substract \(\abs{y}\) from both sides of the above inequality and we
      obtain the result.
    \end{proof}
  \end{enumerate}
\end{enumerate}
\end{document}
