\input{preamble}

\everymath{\displaystyle}

\begin{document}
    \Prblm{1}{$ \int \frac{x^3+10x^2+33x+36}{x^2+4x+3} \, dx. $}
    {$ \frac{1}{2}x^2 + 6x + 6 \ln |x+1| + C. $}
    
    \begin{align*}
        \int \frac{x^3+10x^2+33x+36}{x^2+4x+3} \, dx
            &= \int \paren{x+6+\frac{6}{x+1}} \, dx \\
            &= \frac{x^2}{2} + 6x + 6 \ln|x+1| + C.
    \end{align*}
    
    \Prblm{2}{$ \int \frac{x+2}{(x-1)^2} \, dx. $}
    {$ \ln|x-1| - \frac{3}{x-1} + C. $}
    
    \begin{align*}
        \int \frac{x+2}{(x-1)^2} \, dx
            &= \int \paren{\frac{A}{x-1} + \frac{B}{(x-1)^2}} \, dx \\
            &\deduce \\
        A(x-1) &+ B = x+2 \\
            &\deduce \\
        A = 1 &\quad B = 3 \\
            &\deduce \\
        \int \frac{x+2}{(x-1)^2} \, dx
            &= \int \paren{\frac{1}{x-1} + \frac{3}{(x-1)^2}} \, dx \\
            &= \ln|x-1| - \frac{3}{x-1} + C.
    \end{align*}
    
    \Prblm{3}{$ \int \frac{dx}{x^4 - 6x^3 + 12x^2} $}
    {}
    
    \begin{align*}
        \int \frac{dx}{x^4 - 6x^3 + 12x^2}
            &= \int \frac{dx}{x^2(x^2 - 6x + 12)} \\
            &= \int \paren{\frac{A}{x} + \frac{B}{x^2}
                                       + \frac{Cx+D}{x^2 - 6x + 12}} \, dx \\
            &\deduce \\
        Ax(x^2 - 6x + 12) +{} &B(x^2 - 6x + 12) + (Cx+D)x^2 = 1 \\
            &\deduce \\
        &\hspace{-1in}\left\{\begin{aligned}
              &A && & {}+{} &C && &&= 0 \\
            -6&A & {}+\phantom{12} &B && &{}+{}&D &&= 0 \\
            12&A & {}-\phantom{1}6 &B && && &&= 0 \\
              &  & 12 &B && && &&= 1
        \end{aligned}\,\middle|
        \begin{aligned}
            x^3 \\ x^2 \\ x^1 \\ x^0
        \end{aligned}\right. \\
            &\deduce \\
        A=\frac1{24} \quad B=\frac{1}{12}
            &\quad C=-\frac1{24} \quad D=\frac16 \\
            &\deduce
    \end{align*}
    
    \begin{align*}
        \int \frac{dx}{x^4 - 6x^3 + 12x^2}
            &= \frac1{24}\ln|x| - \frac1{12x}
                    - \frac1{24} \int \frac{x-4}{(x-3)^2+3} \, dx \\
            &\deduce \\
        \int \frac{x-4}{(x-3)^2+3} \, dx
            &= \int \frac{(\sqrt3\tan\theta-1)\cancel{\sqrt3\sec^2\theta}}
                         {\cancelto{\sqrt3}{3\sec^2\theta}} \, d\theta
                &&\hspace{-0.7in}\reason{Let $ x=\sqrt3\tan\theta + 3 $} \\
            &= \int \paren{\tan\theta - \frac1{\sqrt3}} \, d\theta \\
            &= \int \tan\theta \, d\theta - \frac{\theta}{\sqrt3} \\
            &\deduce \\
        \int \tan\theta \, d\theta
            &= \int \frac{\sin\theta}{\cos\theta} \, dx \\
            &= -\int \frac{d\cos\theta}{\cos\theta} \\
            &= -\ln|\cos\theta| + C \\
            &\deduce \\
        \int \frac{x-4}{(x-3)^2+4} \, dx
            &= -\ln|\cos\theta| - \frac{\theta}{\sqrt3} + C\\
            &= -\ln\abs{\cos\paren{\arctan\frac{x-3}{\sqrt3}}}
                   - \frac{1}{\sqrt3}\arctan\frac{x-3}{\sqrt3} + C
                &&\hspace{-0.7in}\reason{$ \theta=\arctan\frac{x-3}{\sqrt3} $} \\
            &= \frac12 \ln\paren{\paren{\frac{x-3}{\sqrt3}}^2 + 1}
                   - \frac{1}{\sqrt3}\arctan\frac{x-3}{\sqrt3} + C
                &&\hspace{-0.7in}\reason{$ \cos(\arctan z) = 1/\sqrt{x^2+1} $} \\
            &= \frac12 \ln(x^2-6x+12)
                    - \frac{1}{\sqrt3} \arctan\frac{x-3}{\sqrt3} + C
                &&\hspace{-0.7in}\reason{$ -\ln3 $ is absorbed by $ C $} \\
            &\deduce \\
        \int \frac{dx}{x^4 - 6x^3 + 12x^2}
            &= \frac1{24}\left[ \ln|x| - \frac2x - \frac12 \ln(x^2-6x+12)
                     + \frac{1}{\sqrt3} \arctan\frac{x-3}{\sqrt3}  \right] + C.
    \end{align*}
\end{document}