\documentclass[a4paper]{book}

\title{Solutions to Graph Theory with Applications}
\author{L. F. \textsc{Jaw}}

\input{preamble-all}
\input{preamble-en}

\makeatletter
\renewenvironment{proof}[1][\proofname]{\par
  \pushQED{\qed}%
  \normalfont \topsep6\p@\@plus6\p@\relax
  \trivlist
  \item[]\ignorespaces
}{%
  \popQED\endtrivlist\@endpefalse
}
\makeatother

\input{preamble-begin}

\begin{document}
\frontmatter
\maketitle

This is a collection of personal solutions to \textit{Graph theory
  with Applications} by Bondy and Murty.

% \tableofcontents
\mainmatter

\chapter{Graphs and Subgraphs}
\label{chap:1}

\section{Graphs and Simple Graphs}
\label{sec:1.1}

\section{Graph Isomorphism}
\label{sec:1.2}

\begin{enumerate}
  \setcounter{enumi}{7}
\item
  \begin{enumerate}
  \item
    \begin{proof}
      The set of vertices of \(K_{m,n}\) can be partitioned into two
      sets \(X\) and \(Y\), where \(\abs{X} = m\) and \(\abs{Y} = n\).
      Since \(K_{m,n}\) is also simple, we have
      \(E(K_{m,n}) = X \times Y\).  It follows that
      \[
        \varepsilon = \abs{E(K_{m,n})} = \abs{X \times Y} = \abs{X} \cdot \abs{Y} = mn. \qedhere
      \]
  \end{proof}
    
  \item
    \begin{proof}
      For any simple and bipartite graph \(G\), which can be
      partitioned into \(X\) and \(Y\), we always have
      \(\varepsilon \le \varepsilon(K_{m,n})\), where \(m = \abs{X}\)
      and \(n = \abs{Y}\).  Since \(\nu = m+n\), for any bipartition
      \((X, Y)\), we have
      \begin{align*}
        \varepsilon &\le \max \varepsilon(K_{m,n}) \\
                    &= \max m(\nu-m) \\
                    &= \frac{\nu}{2} \paren[\Big]{\nu - \frac{\nu}{2}}
                      = \frac{\nu^2}{4}. \qedhere
      \end{align*}
    \end{proof}
  \end{enumerate}
  
\item
  \begin{enumerate}
  \item
    \begin{proof}
      When \(n = m\), we have \(T_{m,n} = T_{m,m} = K_m\) and \(k = \brkt{n/m} = \brkt{m/m} = 1\).  Thus, 
      \begin{align*}
        \binom{n-k}{2} + (m-1) \binom{k+1}{2}
          &= \frac{(m-1)(m-2)}{2} + (m-1) \\
          &= \frac{(m-1)m}{2}
            = \binom{m}{2} \\
          &= \varepsilon(K_m)
            = \varepsilon(T_{m,n}).
      \end{align*}
      This is our induction base.  Suppose now the formula holds for
      some \(1 \le m \le n\).  Let \(k = \brkt{n/m}\).  Then
      \begin{align*}
        \varepsilon(T_{m,n+1})
          &= \varepsilon(T_{m,n}) + k(m-1) + (n+1 - km -1) \\
          &= \varepsilon(T_{m,n}) + n - k \\
          &= \binom{n-k}{2} + (m-1) \binom{k+1}{2} + n - k \\
          &= \frac{(n-k)(n-k-1)}{2} + n - k + (m-1) \binom{k+1}{2} \\
          &= \frac{(n-k)(n-k+1)}{2} + (m-1) \binom{k+1}{2} \\
          &= \binom{n+1-k}{2} + (m-1) \binom{k+1}{2}. \qedhere
      \end{align*}
      Notice that the choice of \(k\) is subtle here.
    \end{proof}
  \item
    \begin{proof}
      Let \(G\) be a complete \(m\)-partite graph on \(n\) vertices.
      Let \(n_1, n_2, \dotsc, n_m\) denote the size of the partitions
      for \(G\).  If \(\abs{n_i - n_j} \le 1\) for all \(i\) and \(j\),
      then \(G \cong T_{m,n}\).  The contrapositive of the previous
      proposition says if \(G \ncong T_{m,n}\), then there exist a pair
      \(i\) and \(j\) such that \(n_i - n_j > 1\).  Then we modify the
      graph \(G\) such that the \(i\)th partition one less vertex and
      the \(j\)th partition has one more vertex.  Outside the two
      partition concerned, the \emph{number} of edges is unchanged.
      Within the two partition concerned, the change of number of edges
      is
      \begin{align*}
        (n_i - 1)(n_j + 1) - n_i n_j
          &= n_i n_j + n_i - n_j - 1 - n_i n_j \\
          &= n_i - n_j - 1 \\
          &> 0.
      \end{align*}
      This completes the proof.
  \end{proof}
  \end{enumerate}
\end{enumerate}

\newpage
\null
\end{document}

